Renaming

GCD.dfy
@@ -75,64 +75,64 @@ lemma ModMultipleIsZero(c: nat)
 	MultiplyThenDivideIsId();
 }
 
-function RemaindersN(a: nat, b: nat): int
+function N(a: nat, b: nat): int
 	requires a > 0
 	decreases b
-	ensures RemaindersN(a, b) >= -1
+	ensures N(a, b) >= -1
 {
 	if b == 0 then -1
-	else 1 + RemaindersN(b, a % b)
+	else 1 + N(b, a % b)
 }
 
-function RemainderK(a: nat, b: nat, k: int): nat
+function R_k(a: nat, b: nat, k: int): nat
 	requires a > 0
-	requires -2 <= k <= RemaindersN(a, b)
+	requires -2 <= k <= N(a, b)
 	decreases b
 {
 	if k == -2 then a
 	else if k == -1 then b
 	else if b == 0 then a
-	else RemainderK(b, a % b, k - 1)
+	else R_k(b, a % b, k - 1)
 }
 
 lemma {:verify false} RemainderK_WhenZeroSpecification(a: nat, b: nat)
 	requires a > 0 && b > 0
-	ensures RemainderK(a, b, RemaindersN(a, b)) == 0
-	ensures forall k : nat :: k < RemaindersN(a, b) ==> RemainderK(a, b, k) > 0
+	ensures R_k(a, b, N(a, b)) == 0
+	ensures forall k : nat :: k < N(a, b) ==> R_k(a, b, k) > 0
 {
 }
 
 // lemma {:verify false} RemainderK_WhenZeroIff(a: nat, b: nat)
 // 	requires a > 0 && b > 0
-// 	ensures forall k : nat :: k == RemaindersN(a, b) <==> RemainderK(a, b, k) == 0
-// 	// ensures k == RemaindersN(a, b) + 1 <==> RemainderK(a, b, k - 1) == 0
+// 	ensures forall k : nat :: k == N(a, b) <==> R_k(a, b, k) == 0
+// 	// ensures k == N(a, b) + 1 <==> R_k(a, b, k - 1) == 0
 // {
 // }
 
 lemma {:verify false} RemaindersN_NonNegative(a: nat, b: nat)
 	requires a > 0 && b > 0
-	ensures RemaindersN(a, b) >= 0
+	ensures N(a, b) >= 0
 {
 }
 
 lemma {:verify false} K_LessThan_N(a: nat, b: nat, k: nat)
 	requires a > 0 && b > 0
-	requires 0 <= k <= RemaindersN(a, b) + 1
-	requires r_k_m1_neq_0: RemainderK(a, b, k - 1) != 0
-	ensures k + 1 <= RemaindersN(a, b) + 1
+	requires 0 <= k <= N(a, b) + 1
+	requires r_k_m1_neq_0: R_k(a, b, k - 1) != 0
+	ensures k + 1 <= N(a, b) + 1
 {
 }
 
 lemma {:verify false} NextRemainerK(a: nat, b: nat, k: int)
 	requires a > 0 && b > 0
-	requires 0 <= k <= RemaindersN(a, b)
-	ensures RemainderK(a, b, k) == RemainderK(a, b, k - 2) % RemainderK(a, b, k - 1)
+	requires 0 <= k <= N(a, b)
+	ensures R_k(a, b, k) == R_k(a, b, k - 2) % R_k(a, b, k - 1)
 {
 }
 
 lemma {:verify false} RemainderNm1IsGcd(a: nat, b: nat)
 	requires a > 0 && b > 0
-	ensures GreatestCommonDivisor(a, b, RemainderK(a, b, RemaindersN(a, b) - 1))
+	ensures GreatestCommonDivisor(a, b, R_k(a, b, N(a, b) - 1))
 {
 }
 
@@ -143,48 +143,42 @@ method ComputeGCD(a: nat, b: nat) returns (i: nat)
 	// k counts the iteration number (starts with 0, zero-based).
 	// r_-2 == a, r_-1 == b
 	ghost var k : nat := 0;
-	ghost var N : int := RemaindersN(a, b);
+	ghost var N : int := N(a, b);
 	var r_k_m2 := a;
 	var r_k_m1 := b;
 
 	RemaindersN_NonNegative(a, b);
 	while (r_k_m1 != 0)
 		invariant k <= N + 1
-		invariant r_k_m2 == RemainderK(a, b, k - 2)
-		invariant r_k_m1 == RemainderK(a, b, k - 1)
+		invariant r_k_m2 == R_k(a, b, k - 2)
+		invariant r_k_m1 == R_k(a, b, k - 1)
 		decreases r_k_m1
 	{
 		K_LessThan_N(a, b, k);
 		NextRemainerK(a, b, k);
 		assert k + 1 <= N + 1;
-		assert r_k_m1 == RemainderK(a, b, (k + 1) - 2);
-		assert r_k_m2 % r_k_m1 == RemainderK(a, b, (k + 1) - 1);
+		assert r_k_m1 == R_k(a, b, (k + 1) - 2);
+		assert r_k_m2 % r_k_m1 == R_k(a, b, (k + 1) - 1);
 
 		r_k_m1, r_k_m2 := r_k_m2 % r_k_m1, r_k_m1;
 
 		assert k + 1 <= N + 1;
-		assert r_k_m2 == RemainderK(a, b, (k + 1) - 2);
-		assert r_k_m1 == RemainderK(a, b, (k + 1) - 1);
+		assert r_k_m2 == R_k(a, b, (k + 1) - 2);
+		assert r_k_m1 == R_k(a, b, (k + 1) - 1);
 
 		k := k + 1;
 		
 		assert k <= N + 1;
-		assert r_k_m2 == RemainderK(a, b, k - 2);
-		assert r_k_m1 == RemainderK(a, b, k - 1);
+		assert r_k_m2 == R_k(a, b, k - 2);
+		assert r_k_m1 == R_k(a, b, k - 1);
 	}
 
 	assert k == N + 1 by {
-		assert r_k_m1 == RemainderK(a, b, k - 1) == 0;
 		RemainderK_WhenZeroSpecification(a, b);
 	}
 	assert GreatestCommonDivisor(a, b, r_k_m2) by {
 		RemainderNm1IsGcd(a, b);
 	}
 
-	// assert k == N;
-	// assert r_k_m3 == RemainderK(a, b, N - 3) && r_k_m2 == RemainderK(a, b, N - 2) && r_k_m1 == RemainderK(a, b, N - 1);
-	// // assert exists q_k : nat :: r_k_m3 == q_k*r_k_m2 + r_k_m1;
-	// assert r_k_m1 == 0;
-	// assert r_k_m3 % r_k_m2 == r_k_m1 == 0;
 	i := r_k_m2;
 }
